Abstract ABD example further to make accesses fully atomic
By abstracting 'Begin' slightly, we can make 'Begin' a right-
and 'End' a left-mover. This allows to make the accesses
fully atomic.
Remove the manual linearizability proof.

Test/civl/samples/ABD.bpl
@@ -12,54 +12,9 @@ This protocol implements two operations Read and Write on a single register
 that is replicated for fault-tolerance and shared across a collection of clients.
 These operations are expected to provide a linearizable interface.
 
-The Civl proof imposes the following abstraction on a detailed protocol specification.
-This abstraction is proved linearizable informallyn but precisely towards
-the end of this file.  
-
-type TimeStamp  // a set with a total order
-TS: TimeStamp   // global timestamp used to order operations
-value_store: Map TimeStamp Value // store for timestamped values
-
-// ReadClient is a wrapper procedure around the Read atomic operation.
-// WriteClient is a wrapper procedure around the Write atomic operation.
-// Begin and End are atomic operations used to mark the start and end of ReadClient and WriteClient.
-// These markers are useful in specifying the linearizability of ReadClient and WriteClient.
-
-ReadClient(one_pid) {
-    old_ts := Begin(one_pid)
-    <yield>
-    ts, val := Read(one_pid, old_ts)
-    <yield>
-    End(one_pid, ts);
-}
-
-WriteClient(one_pid) {
-    old_ts := Begin(one_pid)
-    <yield>
-    ts := Write(one_pid, old_ts)
-    <yield>
-    End(one_pid, ts);
-}
-
-Begin(one_pid) returns (ts) {
-    ts = TS;
-}
-
-Read(one_pid, old_ts) returns (ts, val) {
-    assume old_ts <= ts
-    assume ts in value_store
-    val := value_store[ts]
-}
-
-Write(one_pid, val) returns (ts) {
-    assume old_ts < ts
-    assume ts not in value_store
-    value_store[ts] := val
-}
-
-End(one_pid, ts) {
-    TS := max(TS, ts)
-}
+The Civl proof imposes an abstraction on a detailed protocol specification
+in which the actions READCLIENT and WRITECLIENT represent the atomic operations
+on the register.
 */
 
 //////////////////////////////////////////////////////////////////////////
@@ -116,10 +71,10 @@ function {:inline} le(ts1: TimeStamp, ts2: TimeStamp) : bool {
 //////////////////////////////////////////////////////////////////////////
 // Global variables
 
-var {:layer 1, 4} value_store: Map TimeStamp Value; // unified store of timestamped values shared across all replicas
+var {:layer 1, 5} value_store: Map TimeStamp Value; // unified store of timestamped values shared across all replicas
 var {:layer 1, 3} replica_ts: [ReplicaId]TimeStamp; // projection of replica_store to only the timestamps
 var {:layer 1, 1} last_write: [ProcessId]int;   // last_write[pid] is the version number of the last write by process pid
-var {:layer 0, 4} TS: TimeStamp;    // global timestamp used in the linearizability proof of the abstract protocol
+var {:layer 0, 5} TS: TimeStamp;    // global timestamp used in the linearizability proof of the abstract protocol
 var {:layer 0, 1} replica_store: [ReplicaId]StampedValue;   // state for concrete protocol
 
 /*
@@ -193,6 +148,7 @@ preserves call ReplicaInv();
 preserves call ValidTimeStamp();
 preserves call TimeStampQuorum();
 preserves call ValueStoreInv#3(LeastTimeStamp(), InitValue);
+refines READCLIENT;
 {
     var old_ts: TimeStamp;
     var ts: TimeStamp;
@@ -201,10 +157,21 @@ preserves call ValueStoreInv#3(LeastTimeStamp(), InitValue);
     var {:layer 2} tsq': ReplicaSet;
 
     call old_ts, tsq := Begin(one_pid) | ValueStoreInv#1(LeastTimeStamp(), InitValue) | ValidTimeStamp() | ValueStoreInv#3(LeastTimeStamp(), InitValue);
-    call Yield#4();
     call ts, value, tsq' := Read(one_pid, old_ts, tsq);
-    call Yield#4();
     call End(one_pid, ts);
+}
+
+action {:layer 5} READCLIENT({:linear} one_pid: One ProcessId) returns (value: Value)
+{
+    var old_ts: TimeStamp;
+    var ts: TimeStamp;
+    // tsq is the quorum witnessing the global timestamp TS
+    var {:layer 2, 3} tsq: ReplicaSet;
+    var {:layer 2} tsq': ReplicaSet;
+
+    call old_ts := BEGIN#4(one_pid); // | ValueStoreInv#1(LeastTimeStamp(), InitValue) | ValidTimeStamp() | ValueStoreInv#3(LeastTimeStamp(), InitValue);
+    call ts, value := READ#4(one_pid, old_ts);
+    call End#4(one_pid, ts);
 }
 
 // lwq is the quorum witnessing the last write
@@ -217,6 +184,7 @@ ensures call LastWriteInv(one_pid, ts);
 preserves call ValidTimeStamp();
 preserves call TimeStampQuorum();
 preserves call ValueStoreInv#3(LeastTimeStamp(), InitValue);
+refines WRITECLIENT;
 {
     var old_ts: TimeStamp;
     // tsq is the quorum witnessing the global timestamp TS
@@ -224,16 +192,25 @@ preserves call ValueStoreInv#3(LeastTimeStamp(), InitValue);
     var {:layer 2} tsq': ReplicaSet;
 
     call old_ts, tsq := Begin(one_pid) | ValidTimeStamp() | ValueStoreInv#3(LeastTimeStamp(), InitValue);
-    call Yield#4();
     call ts, lwq', tsq' := Write(one_pid, value, old_ts, lwq, tsq);
-    call Yield#4();
     call End(one_pid, ts);
 }
 
-yield procedure {:layer 3} Begin({:linear} one_pid: One ProcessId) returns (ts: TimeStamp, {:hide} {:layer 2, 3} tsq: ReplicaSet)
-refines action {:layer 4} _ {
-    ts := TS;
+action {:layer 5} WRITECLIENT({:linear} one_pid: One ProcessId, value: Value)
+    returns (ts: TimeStamp)
+{
+    var old_ts: TimeStamp;
+    // tsq is the quorum witnessing the global timestamp TS
+    var {:layer 2, 3} tsq: ReplicaSet;
+    var {:layer 2} tsq': ReplicaSet;
+
+    call old_ts := BEGIN#4(one_pid);
+    call ts := WRITE#4(one_pid, value, old_ts);
+    call End#4(one_pid, ts);
 }
+
+yield procedure {:layer 3} Begin({:linear} one_pid: One ProcessId) returns (ts: TimeStamp, {:hide} {:layer 2, 3} tsq: ReplicaSet)
+refines BEGIN#4;
 preserves call ReplicaInv();
 preserves call ValidTimeStamp();
 ensures call MonotonicInduction#2(tsq, ts, 0);
@@ -243,13 +220,13 @@ ensures {:layer 3} IsQuorum(tsq);
     call ts, tsq := Begin#2(one_pid);
 }
 
+right action {:layer 4,5} BEGIN#4({:linear} one_pid: One ProcessId) returns (ts: TimeStamp) {
+    assume le(ts, TS);
+}
+
 yield procedure {:layer 3} Read({:linear} one_pid: One ProcessId, old_ts: TimeStamp, {:hide} {:layer 2, 3} tsq: ReplicaSet)
     returns (ts: TimeStamp, value: Value, {:hide} {:layer 2} tsq': ReplicaSet)
-refines action {:layer 4} _ { 
-    assume le(old_ts, ts);
-    assume Map_Contains(value_store, ts);
-    value := Map_At(value_store, ts);
-}
+refines READ#4;
 preserves call ValueStoreInv#1(LeastTimeStamp(), InitValue);
 preserves call ReplicaInv();
 preserves call MonotonicInduction#2(tsq, old_ts, 0);
@@ -267,14 +244,18 @@ preserves call ValueStoreInv#3(LeastTimeStamp(), InitValue);
     call tsq' := UpdatePhase(ts, value) | MonotonicInduction#2(tsq, old_ts, 0) | ValidTimeStamp() | ValueStoreInv#1(LeastTimeStamp(), InitValue);
 }
 
+right action {:layer 4,5} READ#4({:linear} one_pid: One ProcessId, old_ts: TimeStamp)
+    returns (ts: TimeStamp, value: Value)
+{
+    assume le(old_ts, ts);
+    assume Map_Contains(value_store, ts);
+    value := Map_At(value_store, ts);
+}
+
 yield procedure {:layer 3}
 Write({:linear} one_pid: One ProcessId, value: Value, old_ts: TimeStamp, {:hide} {:layer 1} lwq: ReplicaSet, {:hide} {:layer 2, 3} tsq: ReplicaSet)
     returns (ts: TimeStamp, {:hide} {:layer 1} lwq': ReplicaSet, {:hide} {:layer 2} tsq': ReplicaSet)
-refines action {:layer 4} _ {
-    assume lt(old_ts, ts);
-    assume !Map_Contains(value_store, ts);
-    value_store := Map_Update(value_store, ts, value);
-}
+refines WRITE#4;
 requires call MonotonicInduction#1(lwq, TimeStamp(last_write[one_pid->val], one_pid->val), 0);
 ensures call MonotonicInduction#1(lwq', ts, 0);
 requires call LastWriteInv(one_pid, TimeStamp(last_write[one_pid->val], one_pid->val));
@@ -298,6 +279,14 @@ preserves call ValueStoreInv#3(LeastTimeStamp(), InitValue);
     call q := UpdatePhase(ts, value) | LastWriteInv(one_pid, ts) | MonotonicInduction#2(tsq, old_ts, 0) | ValidTimeStamp();
     lwq' := q;
     tsq' := q;
+}
+
+action {:layer 4,5} WRITE#4({:linear} one_pid: One ProcessId, value: Value, old_ts: TimeStamp)
+    returns (ts: TimeStamp)
+{
+    assume lt(old_ts, ts);
+    assume !Map_Contains(value_store, ts);
+    value_store := Map_Update(value_store, ts, value);
 }
 
 yield right procedure {:layer 3} QueryPhase(old_ts: TimeStamp, {:layer 1} old_replica_store: [ReplicaId]StampedValue, {:layer 2, 3} tsq: ReplicaSet)
@@ -534,86 +523,19 @@ refines action {:layer 1} _ {
 }
 
 yield procedure {:layer 0} End({:linear} one_pid: One ProcessId, ts: TimeStamp);
-refines action {:layer 1, 4} _ {
+refines End#3;
+
+action {:layer 1, 3} End#3({:linear} one_pid: One ProcessId, ts: TimeStamp)
+refines End#4;
+{
     if (lt(TS, ts)) {
         TS := ts;
     }
 }
 
-/*
-We prove that the last layer shown below is linearizable.
+left action {:layer 4,5} End#4({:linear} one_pid: One ProcessId, ts: TimeStamp) {
+    if (lt(TS, ts)) {
+        TS := ts;
+    }
+}
 
-// Definition of <HB
-Given any concurrent execution, we define a happens-before order (<HB) as follows:
-op1 <HB op2 iff End of op1 executes before Begin of op2. We have the following two lemmas about <HB.
-
-// HB_Lemma 1: <HB is a strict partial order
-The proof follows from the totally-ordered nature of a concurrent execution.
-
-// HB_Lemma 2: if op1 <HB op2, then op1.ts <= op2.ts
-  Case 1: op2 is a write
-          From the specification "assume old_ts < ts" for writes, we have op1.ts < op2.ts
-  Case 2: op2 is a read
-          From the specification "assume old_ts <= ts" for reads, we have op1.ts <= op2.ts
-
-// Definition of <L
-Given any concurrent execution, we construct a linearization order (<L) of ReadClient and WriteClient operations
-that is a correct sequential specification of an atomic register and is consistent with <HB.
-We associate WriteClient and ReadClient with the ts that is calculated in their Write and Read actions, respectively.
-From this point on, we'll refer to WriteClient and ReadClient operations simply as write and read,
-and write.ts and read.ts to refer to their associated timestamp.
-
-Order op1 <L op2: 
-C1. if op1.ts < op2.ts, or
-C2. if op1.ts == op2.ts and op1 is a write and op2 is a read, or
-C3. if op1.ts == op2.ts and both are reads and op1 <HB op2 
-
-// <L is a strict partial order
-Irreflexive: not(op <L op)
-op.ts < op.ts is not possible
-op can't be both a read and a write 
-op <HB op is not possible (since <HB is a strict partial order)
-
-Asymmetry: if op1 <L op2,  then not(op2 <L op1)
-Case 1: op1.ts < op2.ts => not(op2.ts < op1.ts) and not(op2.ts == op1.ts), therefore we have not(op2 <L op1)
-Case 2: op1.ts == op2.ts
-        Case 2.1: op1 is a write and op2 is a read
-                  therefore we have not(op2 <L op1)
-        Case 2.2: op1 is a read and op2 is a read
-                  since op1 <L op2, we must have op1 <HB op2, which implies not(op2 <HB op1) (since <HB is a strict partial order)
-                  therefore we have not(op2 <L op1)
-
-Transitivity: if op1 <L op2 and op2 <L op3,  then op1 <L op3
-op1.ts <= op2.ts and op2.ts <= op3.ts ==> op1.ts <= op3.ts (transitive property of inequality)
-Case 1: op1.ts < op3.ts then op1 <L op3 (from C1)
-Case 2: op1.ts == op3.ts
-          op1.ts == op3.ts implies op1.ts == op2.ts == op3.ts 
-          Case 2.1: op1 is a write and op2 is a read and op3 is a read
-                    op1.ts == op3.ts and op1 is a write and op3 is a read ==> op1 <L op3 (from C2)
-          Case 2.2: op1 is a read and op2 is a read and op3 is a read
-                    we have op1 <HB op2 <HB op3 => op1 <HB op3 (<HB is a strict partial order)
-                    since op1.ts == op3.ts and op1 <HB < op3, we have op1 <L op3 (from C3)                
-
-// Show that the reads return values consistent with an atomic register
-We prove that in <L every read returns the value written by the last preceding write. 
-From the specification "assume ts is not in value_store" for writes, we get that for any two write operations w1 and w2,
-either w1.ts < w2.ts or w2.ts < w1.ts holds. 
-This implies w1 <L w2 or w2 <L w1 (from C1)
-From the specification "assume ts in value_store" for reads, we get that any read r reads something that is written by some write w.
-Therefore, w.ts == r.ts, which implies w <L r (from C2)
-From the above two points, we can conclude that there exists a subset of <L that forms a total order over all writes and any given read r, as follows: 
-w_0 < ... < w_i < r < w_(i+1) < ... < w_n, where w_i.ts == r.ts
-Since any total order of <L will respect this order among writes and a read, we can conclude that the read returns the value written by the last preceding write.
-
-// Show that <L is consistent with happens before order: op1 <HB op2 ==> op1 <L op2
-we have op1.ts <= op2.ts (from HB_Lemma 2)
-Case 1: op1.ts < op2.ts, then we have op1 <L op2 (from C1)
-Case 2: op1.ts == op2.ts
-     Case 2.1: op1 is a read and op2 is a write
-               But from the specification "assume old_ts < ts" for writes, we must have op1.ts < op2.ts. Therefore, this case is not possible.
-     Case 2.2: op1 is a read and op2 is  aread
-               and we also have op1 <HB op2, which implies op1 <L op2 (from C3)
-     Case 2.3: op1 is a write and op2 is a read
-               we have op1 <L op2 (from C2)
-Therefore, any total ordering of <L will also be consistent with <HB.
-*/
